Is0/Is0.lean
@@ -5,176 +5,79 @@ import Mathlib.Data.ZMod.Basic
 import Mathlib.Tactic.LibrarySearch
 
 import Is0.Basic
+import Is0.Lemmas
 import Is0.Programs
 
 namespace Risc0
 
-lemma Cirgen.step_Sequence_Assign_collapsible :
-  ∀ (state : State) (name : String) (op : Op) (program : Cirgen),
-  Cirgen.step state (.Sequence (.Assign name op) program) = Cirgen.step (state.update name (Op.eval state op)) program := by
-  intros state name op program
-  cases op <;> {
-    conv =>
-      lhs
-      unfold Cirgen.step
-      simp only [State.update, Map.update, beq_iff_eq]
-  }
-
-lemma Cirgen.step_Sequence_Set_collapsible
-    {state : State}
-    {name : String}
-    {nameₓ : String}
-    {program : Cirgen}
-    (buffer : List Felt)
-    (x : Felt)
-    (h : state.buffers name = some buffer)
-    (h₁ : state.felts nameₓ = some x) :
-    Cirgen.step state (.Sequence (.Set (Variable.mk name) i (Variable.mk nameₓ)) program)
-  = let buffers' := state.buffers.update name (buffer.set i x)
-    Cirgen.step ({ state with buffers := buffers' }) program := by
-  conv =>
-    lhs
-    unfold step
-  unfold step
-  simp only [Map.update, beq_iff_eq]
-  rw [h]
-  rw [h₁]
-  done
-
-lemma Cirgen.step_Sequence_If_collapsible
-    {state : State}
-    {name : String}
-    {branch : Cirgen}
-    {program : Cirgen}
-    (x : Felt)
-    (h₁ : state.felts name = some x)
-    (hab : step state program ≠ step state (Sequence branch program))
-    (hhh : (state, none) ≠ step state branch) :
-    Cirgen.step state (.Sequence (.If (Variable.mk name) branch) program)
-  = if (x == 0)
-      then Cirgen.step state program
-      else Cirgen.step state (.Sequence branch program) := by
-  simp only [beq_iff_eq]
-  let a := step state program
-  let b := step state (Sequence branch program)
-  have ha : a = step state program := by simp only
-  have hb : b = step state (Sequence branch program) := by simp only
-  rw [← ha]
-  rw [← hb]
-  by_cases x = 0
-  have hh := (@Ne.ite_eq_left_iff (State × Option Prop) (x = 0) _ a b hab).2 h
-  rw [hh]
-  conv =>
-    lhs
-    unfold step
-    unfold step
-  simp only [beq_iff_eq, Map.update]
-  rw [h₁]
-  simp only
-  have hh₁ := (@Ne.ite_eq_left_iff (State × Option Prop) (x = 0) _ (state, none) (step state branch) hhh).2 h
-  rw [hh₁]
-  simp only
-  conv =>
-    rhs
-    unfold step
-  simp only [beq_iff_eq, Map.update]
-  rw [←ite_not]
-  have hba : b ≠ a := by
-    rw [ha]
-    rw [hb]
-    rw [ne_comm]
-    exact hab
-  have hh := (@Ne.ite_eq_left_iff (State × Option Prop) (¬x = 0) _ b a hba).2 h
-  rw [hh]
-  conv =>
-    lhs
-    unfold step
-    unfold step
-  simp only [beq_iff_eq, Map.update]
-  rw [h₁]
-  simp only
-  rw [←ite_not]
-  have hhhh : step state branch ≠ (state, none) := by
-    rw [ne_comm]
-    exact hhh
-  have hh₁ := (@Ne.ite_eq_left_iff (State × Option Prop) (¬x = 0) _ (step state branch) (state, none) hhhh).2 h
-  rw [hh₁]
-  simp only
-  conv =>
-    rhs
-    unfold step
-  simp only [beq_iff_eq, Map.update]
-  conv in (step (step state branch).fst program) =>
-    unfold step
-  simp only [beq_iff_eq, Map.update]
-
-lemma Cirgen.step_If_collapsible
-    {state : State}
-    {name : String}
-    {branch : Cirgen}
-    (x : Felt)
-    (h₁ : state.felts name = some x) :
-    Cirgen.step state (.If (Variable.mk name) branch)
-  = if (x == 0)
-      then (state, none)
-      else Cirgen.step state branch := by
-  sorry
-
 theorem is0OriginalProgram_constraints_are_what_we_expect :
-  ∀ x y z : Felt, (is0OriginalProgram x y z).1.constraints.foldr And _root_.True ↔ (x = 0 ∧ x * x⁻¹ - 1 = 0) := by
+  ∀ x y z : Felt, (is0OriginalProgram x y z).1.constraints.foldr And _root_.True ↔ (if x == 0 then x = 0 else x * x⁻¹ - 1 = 0) := by
   intros x y z
   unfold is0OriginalProgram
+  by_cases x = 0
+  rw [h]
   rw [Cirgen.step_Sequence_Assign_collapsible]
-  simp only [State.update, Map.empty, Map.fromList, Map.update, beq_iff_eq]
-  unfold Op.eval
-  simp only
+  simp only [List.foldr, and_self]
   rw [Cirgen.step_Sequence_Assign_collapsible]
-  simp only [State.update, Map.empty, Map.fromList, Map.update, beq_iff_eq]
-  unfold Op.eval
-  simp only
+  simp only [State.update, Map.empty, Map.fromList, Map.update, beq_iff_eq, ne_eq]
+  unfold Op.eval ; simp only
   rw [Cirgen.step_Sequence_Assign_collapsible]
-  simp only [State.update, Map.empty, Map.fromList, Map.update, beq_iff_eq]
-  unfold Op.eval
-  simp only [List.getD_cons_zero, ite_false, ite_true, beq_iff_eq, ne_eq]
-  rw [Cirgen.step_Sequence_Set_collapsible [y, z] (if x = 0 then 1 else 0)]
-  simp only
+  simp only [State.update, Map.empty, Map.fromList, Map.update, beq_iff_eq, ne_eq]
+  unfold Op.eval ; simp only
+  unfold List.getD ; unfold List.get? ; unfold Option.getD ; simp only
   rw [Cirgen.step_Sequence_Assign_collapsible]
-  simp only [State.update, Map.empty, Map.fromList, Map.update, beq_iff_eq]
-  unfold Op.eval
-  simp only
-  rw [Cirgen.step_Sequence_Set_collapsible [y, z] (if (x == 0) = true then 0 else x⁻¹)]
-  simp only [beq_iff_eq, Map.update, List.set_succ, ne_eq]
-  rw [Cirgen.step_Sequence_Assign_collapsible]
-  simp only [State.update, Map.empty, Map.fromList, Map.update, beq_iff_eq]
-  unfold Op.eval
-  simp only [ite_true, ite_false, List.getD_cons_zero, ne_eq]
-  rw [Cirgen.step_Sequence_If_collapsible y]
-  rw [Cirgen.step_Sequence_Assign_collapsible]
-  simp only [State.update, Map.empty, Map.fromList, Map.update, beq_iff_eq]
-  unfold Op.eval
-  simp only
-  rw [Cirgen.step_If_collapsible (1 - y)]
+  simp only [State.update, Map.empty, Map.fromList, Map.update, beq_iff_eq, ne_eq]
+  unfold Op.eval ; simp only
   simp only [beq_iff_eq, ne_eq]
+  rw [if_neg h]
+  rw [if_neg h]
+  rw [Cirgen.step_Sequence_Set_collapsible [y, z] 0]
+  simp only [Map.update, beq_iff_eq, ne_eq]
   rw [Cirgen.step_Sequence_Assign_collapsible]
-  simp only [State.update, Map.empty, Map.fromList, Map.update, beq_iff_eq]
-  unfold Op.eval
-  simp only
+  simp only [State.update, Map.update, beq_iff_eq, ne_eq]
+  unfold Op.eval ; simp only
+  unfold List.set
+  simp only [beq_iff_eq, ne_eq]
+  rw [if_neg h]
+  rw [Cirgen.step_Sequence_Set_collapsible [0, z] x⁻¹]
+  simp only [Map.update, beq_iff_eq, List.set_succ, and_true, ne_eq]
   rw [Cirgen.step_Sequence_Assign_collapsible]
-  simp only [State.update, Map.empty, Map.fromList, Map.update, beq_iff_eq]
-  unfold Op.eval
-  simp only
+  simp only [State.update, Map.empty, Map.fromList, Map.update, beq_iff_eq, and_true, ne_eq]
+  unfold Op.eval ; simp only
+  unfold List.getD ; unfold List.get? ; unfold Option.getD ; simp only
+  rw [Cirgen.step_Sequence_If_collapsible 0]
+  unfold List.set
+  simp only [and_true, ne_eq]
   rw [Cirgen.step_Sequence_Assign_collapsible]
-  simp only [State.update, Map.empty, Map.fromList, Map.update, beq_iff_eq]
-  unfold Op.eval
-  simp only
-  sorry
-  sorry
-  sorry
-  sorry
-  sorry
-  sorry
-  sorry
-  sorry
-  sorry
+  unfold Op.eval ; simp only
+  simp only [State.update, Map.update, beq_iff_eq, sub_zero, and_true, ne_eq]
+  rw [ite_true]
+  rw [Cirgen.step_If_collapsible 1]
+  simp only [List.foldr, and_true, ne_eq]
+  nth_rewrite 1 [Op.assign]
+  nth_rewrite 1 [Op.eval]
+  simp only [Map.update, ite_true, Option.some.injEq, ne_eq]
+  nth_rewrite 1 [Op.assign]
+  nth_rewrite 1 [Op.eval]
+  simp only [ite_true, ite_false, List.getD_cons_succ, List.getD_cons_zero, Map.update, beq_iff_eq, Option.some.injEq, ne_eq]
+  nth_rewrite 1 [Op.assign]
+  nth_rewrite 1 [Op.eval]
+  simp only [ite_true, ite_false, List.getD_cons_succ, List.getD_cons_zero, Map.update, beq_iff_eq, ne_eq, Option.some.injEq]
+  nth_rewrite 1 [Op.assign]
+  nth_rewrite 1 [Op.eval]
+  simp only [ne_eq, Map.update, ite_false, Option.some.injEq]
+  nth_rewrite 1 [Op.assign]
+  nth_rewrite 1 [Op.eval]
+  simp only [ne_eq, ite_true, ite_false, List.getD_cons_succ, List.getD_cons_zero, Map.update, beq_iff_eq, ite_self]
+  simp only [ite_false, ite_true]
+  simp only [ite_false, ite_true]
+  apply @hab x y z
+  rw [Cirgen.step_Eqz_collapsible x]
+  simp only [ne_eq, Prod.mk.injEq, State.mk.injEq, and_false, and_true, not_false_iff]
+  simp only [ite_false, ite_true]
+  simp only [ite_false, ite_true]
+  simp only [ite_false, ite_true]
+  simp only [ite_false, ite_true]
+  simp only [ite_false, ite_true]
 
 end Risc0
