Is0/Lemmas.lean
@@ -1,0 +1,246 @@
+import Mathlib.Data.Nat.Prime
+import Mathlib.Data.Vector
+import Mathlib.Data.ZMod.Defs
+import Mathlib.Data.ZMod.Basic
+import Mathlib.Tactic.LibrarySearch
+
+import Is0.Basic
+import Is0.Programs
+
+namespace Risc0
+
+lemma Cirgen.step_Sequence_Assign_collapsible :
+  ∀ (state : State) (name : String) (op : Op) (program : Cirgen),
+  Cirgen.step state (.Sequence (.Assign name op) program) = Cirgen.step (state.update name (Op.eval state op)) program := by
+  intros state name op program
+  cases op <;> {
+    conv =>
+      lhs
+      unfold Cirgen.step
+  }
+
+lemma Cirgen.step_Sequence_Set_collapsible
+    {state : State}
+    {name : String}
+    {nameₓ : String}
+    {program : Cirgen}
+    (buffer : List Felt)
+    (x : Felt)
+    (h : state.buffers name = some buffer)
+    (h₁ : state.felts nameₓ = some x) :
+    Cirgen.step state (.Sequence (.Set (Variable.mk name) i (Variable.mk nameₓ)) program)
+  = let buffers' := state.buffers.update name (buffer.set i x)
+    Cirgen.step ({ state with buffers := buffers' }) program := by
+  conv =>
+    lhs
+    unfold step
+  conv in step state (Set (Variable.mk name) i (Variable.mk nameₓ)) =>
+    unfold step
+  simp only [ne_eq, decide_not]
+  rw [h]
+  rw [h₁]
+
+lemma Cirgen.step_Sequence_If_collapsible
+    {state : State}
+    {name : String}
+    {branch : Cirgen}
+    {program : Cirgen}
+    (x : Felt)
+    (h₁ : state.felts name = some x)
+    (hab : step state program ≠ step state (Sequence branch program))
+    (hhh : (state, none) ≠ step state branch) :
+    Cirgen.step state (.Sequence (.If (Variable.mk name) branch) program)
+  = if (x == 0)
+      then Cirgen.step state program
+      else Cirgen.step state (.Sequence branch program) := by
+  simp only [beq_iff_eq]
+  let a := step state program
+  let b := step state (Sequence branch program)
+  have ha : a = step state program := by simp only
+  have hb : b = step state (Sequence branch program) := by simp only
+  rw [← ha]
+  rw [← hb]
+  by_cases x = 0
+  have hh := (@Ne.ite_eq_left_iff (State × Option Prop) (x = 0) _ a b hab).2 h
+  rw [hh]
+  conv =>
+    lhs
+    unfold step
+    unfold step
+  simp only [beq_iff_eq]
+  rw [h₁]
+  simp only
+  have hh₁ := (@Ne.ite_eq_left_iff (State × Option Prop) (x = 0) _ (state, none) (step state branch) hhh).2 h
+  rw [hh₁]
+  simp only
+  conv =>
+    rhs
+    unfold step
+  simp only [beq_iff_eq]
+  rw [←ite_not]
+  have hba : b ≠ a := by
+    rw [ha]
+    rw [hb]
+    rw [ne_comm]
+    exact hab
+  have hh := (@Ne.ite_eq_left_iff (State × Option Prop) (¬x = 0) _ b a hba).2 h
+  rw [hh]
+  conv =>
+    lhs
+    unfold step
+    unfold step
+  simp only [beq_iff_eq]
+  rw [h₁]
+  simp only
+  rw [←ite_not]
+  have hhhh : step state branch ≠ (state, none) := by
+    rw [ne_comm]
+    exact hhh
+  have hh₁ := (@Ne.ite_eq_left_iff (State × Option Prop) (¬x = 0) _ (step state branch) (state, none) hhhh).2 h
+  rw [hh₁]
+  simp only
+  conv =>
+    rhs
+    unfold step
+  simp only [beq_iff_eq]
+  conv in (step (step state branch).fst program) =>
+    unfold step
+  simp only [beq_iff_eq]
+
+lemma Cirgen.step_If_collapsible
+    {state : State}
+    {name : String}
+    {branch : Cirgen}
+    (x : Felt)
+    (h₁ : state.felts name = some x) :
+    Cirgen.step state (.If (Variable.mk name) branch)
+  = if (x == 0)
+      then (state, none)
+      else Cirgen.step state branch := by
+  conv =>
+    lhs
+    unfold step
+  simp only [beq_iff_eq]
+  rw [h₁]
+  done
+
+lemma Cirgen.step_Eqz_collapsible
+    {state : State}
+    {name : String}
+    (x : Felt)
+    (h₁ : state.felts name = some x) :
+    Cirgen.step state (.Eqz (Variable.mk name))
+  = ({ state with constraints := (x = 0) :: state.constraints }, none) := by
+  conv =>
+    lhs
+    unfold step
+  simp only [beq_iff_eq]
+  rw [h₁]
+  done
+
+lemma Cirgen.step_Sequence_Eqz_collapsible
+    {state : State}
+    {name : String}
+    {program : Cirgen}
+    (x : Felt)
+    (h₁ : state.felts name = some x) :
+    Cirgen.step state (.Sequence (.Eqz (Variable.mk name)) program)
+  = let state₁ := { state with constraints := (x = 0) :: state.constraints }
+    let (state₂, y) := Cirgen.step state₁ program
+    (state₂, y) := by
+  simp only [Prod.mk.eta]
+  conv =>
+    lhs
+    unfold step
+  simp only
+  rw [Cirgen.step_Eqz_collapsible x]
+  exact h₁
+
+lemma hab {x y z : Felt} : Cirgen.step
+    {
+      felts := fun x_1 =>
+        if x_1 = "out[0]" then some 0
+        else
+          if x_1 = "invVal" then some x⁻¹
+          else if x_1 = "isZeroBit" then some 0 else if x_1 = "x" then some x else if x_1 = "1" then some 1 else none,
+      props := fun _ => none,
+      buffers := fun x_1 =>
+        if x_1 = "out" then some (0 :: List.set [z] 0 x⁻¹)
+        else
+          if x_1 = "out" then some [0, z]
+          else if x_1 = "in" then some [x] else if x_1 = "out" then some [y, z] else none,
+      constraints := [] }
+    (Cirgen.Sequence (Cirgen.Assign "1 - out[0]" (Op.Sub (Variable.mk "1") (Variable.mk "out[0]")))
+      (Cirgen.If (Variable.mk "1 - out[0]")
+        (Cirgen.Sequence (Cirgen.Assign "out[1]" (Op.Get (Variable.mk "out") 1 0))
+          (Cirgen.Sequence (Cirgen.Assign "x * out[1]" (Op.Mul (Variable.mk "x") (Variable.mk "out[1]")))
+            (Cirgen.Sequence (Cirgen.Assign "x * out[1] - 1" (Op.Sub (Variable.mk "x * out[1]") (Variable.mk "1")))
+              (Cirgen.Eqz (Variable.mk "x * out[1] - 1"))))))) ≠
+  Cirgen.step
+    {
+      felts := fun x_1 =>
+        if x_1 = "out[0]" then some 0
+        else
+          if x_1 = "invVal" then some x⁻¹
+          else if x_1 = "isZeroBit" then some 0 else if x_1 = "x" then some x else if x_1 = "1" then some 1 else none,
+      props := fun _ => none,
+      buffers := fun x_1 =>
+        if x_1 = "out" then some (0 :: List.set [z] 0 x⁻¹)
+        else
+          if x_1 = "out" then some [0, z]
+          else if x_1 = "in" then some [x] else if x_1 = "out" then some [y, z] else none,
+      constraints := [] }
+    (Cirgen.Sequence (Cirgen.Eqz (Variable.mk "x"))
+      (Cirgen.Sequence (Cirgen.Assign "1 - out[0]" (Op.Sub (Variable.mk "1") (Variable.mk "out[0]")))
+        (Cirgen.If (Variable.mk "1 - out[0]")
+          (Cirgen.Sequence (Cirgen.Assign "out[1]" (Op.Get (Variable.mk "out") 1 0))
+            (Cirgen.Sequence (Cirgen.Assign "x * out[1]" (Op.Mul (Variable.mk "x") (Variable.mk "out[1]")))
+              (Cirgen.Sequence (Cirgen.Assign "x * out[1] - 1" (Op.Sub (Variable.mk "x * out[1]") (Variable.mk "1")))
+                (Cirgen.Eqz (Variable.mk "x * out[1] - 1")))))))) := by
+  unfold List.set
+  rw [Cirgen.step_Sequence_Assign_collapsible]
+  simp only [State.update, Map.update, beq_iff_eq, ne_eq]
+  unfold Op.eval ; simp only [sub_zero]
+  rw [Cirgen.step_If_collapsible 1]
+  simp only [ite_false]
+  rw [Cirgen.step_Sequence_Assign_collapsible]
+  simp only [State.update, Map.update, beq_iff_eq]
+  unfold Op.eval
+  simp only [ite_true, ite_false, List.getD_cons_succ, List.getD_cons_zero]
+  rw [Cirgen.step_Sequence_Assign_collapsible]
+  simp only [State.update, Map.update, beq_iff_eq]
+  unfold Op.eval
+  simp only [ite_false, ite_true, ne_eq]
+  rw [Cirgen.step_Sequence_Assign_collapsible]
+  simp only [State.update, Map.update, beq_iff_eq]
+  unfold Op.eval
+  simp only [ite_false, ite_true, ne_eq]
+  rw [Cirgen.step_Eqz_collapsible (x * x⁻¹ - 1)]
+  simp only
+  rw [Cirgen.step_Sequence_Eqz_collapsible x]
+  simp only [ne_eq, Prod.mk.eta]
+  rw [Cirgen.step_Sequence_Assign_collapsible]
+  simp only [State.update, Map.update, beq_iff_eq]
+  unfold Op.eval
+  simp only [ne_eq, ite_true, ite_false, sub_zero]
+  rw [Cirgen.step_If_collapsible 1]
+  simp only [ite_false]
+  rw [Cirgen.step_Sequence_Assign_collapsible]
+  simp only [State.update, Map.update, beq_iff_eq]
+  unfold Op.eval
+  simp only [ne_eq, ite_true, ite_false, List.getD_cons_succ, List.getD_cons_zero]
+  rw [Cirgen.step_Sequence_Assign_collapsible]
+  simp only [ne_eq, State.update, Map.update, beq_iff_eq]
+  unfold Op.eval ; simp only
+  rw [Cirgen.step_Sequence_Assign_collapsible]
+  simp only [ne_eq, State.update, Map.update, beq_iff_eq]
+  unfold Op.eval ; simp only
+  rw [Cirgen.step_Eqz_collapsible (x * x⁻¹ - 1)]
+  simp only [ne_eq, Prod.mk.injEq, State.mk.injEq, List.cons.injEq, and_false, and_true, not_false_iff]
+  simp only [ite_false, ite_true]
+  simp only [ite_false, ite_true]
+  simp only [ite_false, ite_true]
+  simp only [ite_false, ite_true]
+  simp only [ite_false, ite_true]
+
+end Risc0
